PolyFun/PFunctor/Cofree.lean
@@ -159,6 +159,9 @@ instance : LawfulComonad (CofreeC F) where
   coseq_assoc := by
     intro α β γ wa wb wc
     simp [coseq, Functor.map, Function.comp, extend_assoc]
+  map_coseq := by
+    intro α β α' β' f g wa wb
+    simp [coseq, Functor.map, Function.comp, extend_assoc]
   map_eq_extend_extract := by
     intro α β f t
     rfl
